\documentclass{article}

\usepackage{amsmath}
\usepackage{amsfonts}

\newcommand{\E}{\mathbb{E}}
\newcommand{\rX}{\mathsf{X}}
\newcommand{\rY}{\mathsf{Y}}
\newcommand{\Var}{\text{Var}}

\begin{document}

\section{a}

$$\E[\rX]$$
$$=\E[\sum_i \rX_i]$$
$$=\sum_i \E[\rX_i]$$
$$= n \E[\rX_i]$$
$$= n \frac{1}{p}$$

\

$$\Var(\rX)$$
$$= \Var(\sum_i \rX_i)$$
$$= \sum_i \Var(\rX_i)$$
$$= n \Var(\rX_i)$$
$$= n \frac{1-p}{p^2}$$

\section{b}

$$\Pr[|\rX - \E[\rX]| \geq \epsilon] \leq \frac{\Var(\rX)}{\epsilon ^2}$$

$$\Pr[|\rX - \frac{n}{p}| \geq \epsilon] \leq \frac{n \frac{1-p}{p^2}}{\epsilon ^2}$$

$$\Pr[|\rX - \frac{n}{p}| \geq \epsilon] \leq \frac{n \frac{1-p}{p^2}}{\epsilon ^2}$$

$$\Pr[\rX \geq (1+(n\frac{1-p}{p^2}))\frac{n}{p}] \leq
\frac{1}{(n\frac{1-p}{p^2})\frac{n}{p}}$$

$$\Pr[\rX \geq (\frac{p^2+n-np}{p^2})\E[\rX]] \leq
\frac{p^3}{n^3-n^2p}$$

$$c = $$

\end{document}
